new ssreflect version, Makefile fixes, MN WIP

myhill_nerode.v
@@ -2,6 +2,10 @@ Require Import ssreflect ssrbool ssrnat fintype eqtype seq ssrfun ssrbool finset
 Require Import automata misc regexp.
 Require Import Program.Equality.
 
+Require Import base.
+
+Set Implicit Arguments.
+
 Section MyhillNerode.
   Variable char: finType.
   Definition word:= word char.
@@ -10,7 +14,7 @@ Section MyhillNerode.
     Variable X: finType.
     Variable L: language char.
 
-    Definition MH_rel w1 w2 := forall w3, w1++w3 \in L <-> w2++w3 \in L.
+    Definition MN w1 w2 := forall w3, w1++w3 \in L <-> w2++w3 \in L.
 
     (* We model finiteness of equivalence classes
      by functions to some finType. *)
@@ -19,7 +23,10 @@ Section MyhillNerode.
     
     (* We define what it means to be a refinement
      of the MH relation: *)
-    Definition MH_rel_ref (f: Fin_eq_cls) := forall w1 w2, f w1 = f w2 <-> MH_rel w1 w2.
+    Definition MN_rel (f: Fin_eq_cls) := forall w1 w2, f w1 = f w2 <-> MN w1 w2.
+
+    (* We also define refinements of the MN relation *)
+    Definition MN_ref (f: Fin_eq_cls) := forall w1 w2, f w1 = f w2 -> MN w1 w2.
     
   End Relation.
 
@@ -27,7 +34,7 @@ Section MyhillNerode.
     Variable L: language char.
     Variable X: finType.
     Variable f: Fin_eq_cls X.
-    Variable ref: MH_rel_ref X L f.
+    Variable ref: MN_rel L f.
 
     Definition surj (f: Fin_eq_cls X) := forall x, exists w, f(w) == x. 
 
@@ -43,20 +50,12 @@ Section MyhillNerode.
     
     Definition repr := [ fun w => f_inv (f w) ].
                                          
-    Lemma f_inv_inj: injective f_inv.
-    Proof.
-      move => x y.
-      move: (xchooseP (f_surj x)) => /eqP {2}<-.
-      move: (xchooseP (f_surj y)) => /eqP {2}<-.
-      by rewrite /f_inv => ->.
-    Qed.
-
     Lemma f_inv_invariant_rcons w a: f (rcons (f_inv (f w)) a) = f (rcons w a).
     Proof.
       apply ref.
       move => z.
       rewrite -2!cats1 -2!catA /=. pattern (a::z).
-      assert (MH_rel L (f_inv (f w)) w).
+      assert (MN L (f_inv (f w)) w).
         apply ref.
         by rewrite f_invK.
       exact: H.
@@ -103,11 +102,74 @@ Section MyhillNerode.
       
   End ToDFA.
 
+  Section Minimalization.
+    Variable L: language char.
+    Variable X: finType.
+    Variable f: Fin_eq_cls X.
+    Variable ref: MN_ref L f.
+    Variable f_surj: surj f.
+
+    Record MState :=
+      mstateI {
+          todo: seq (X*X);
+          disjunct: {set X*X}
+      }.
+
+    Definition ext x y a := (f (rcons (f_inv f_surj x) a), f (rcons (f_inv f_surj y) a)). 
+    Definition dist_ext1 x y a:= f (rcons (f_inv f_surj x) a) != f (rcons (f_inv f_surj y) a).
+
+    Definition dist_extS x y w := f (cat (f_inv f_surj x) w) != f (cat (f_inv f_surj y) w).
+
+    
+
+    Definition propagate x y disjunct :=
+      disjunct :|: [ set x' | (x,y) \in [ set ext (fst x') (snd x') a | a <- char ]  ].
+
+    Lemma propagate_monotone (disjunct: {set X*X}) x y: disjunct \subset (propagate x y disjunct). 
+    Proof.
+      by apply: subsetUl.
+    Qed.
+
+    Fixpoint unnamed1 todo  :=
+      match todo with
+      | [::] => set0: {set X*X}
+      | ((x,y)::todo) =>
+          if x == y then unnamed1 todo else  
+          match [ pick a | dist_ext1 x y a ] with
+          | None => unnamed1 todo
+          | Some a => let r := unnamed1 todo in
+                        r :|: (mu (propagate x y)) 
+          end
+      end.
+
+    Section Correctness.
+      Definition reflexive (S: {set X*X}):= forall x y, (x,y) \in S -> (y,x) \in S.
+      
+      Lemma unnamed1_final todo x y: (x,y) \in  unnamed1 todo -> exists a, dist_ext1 x y a. 
+      Proof.
+        elim: todo => [|[x' y'] todo IHtd].          
+          by rewrite /= in_set0.
+        rewrite /=.
+        case H0: (x' == y') => //.
+        case: pickP => a H.
+          rewrite /= in_setU => /orP [] //.
+
+          eapply mu_ind => [|s IHs].
+            rewrite in_set0 //.
+          rewrite in_setU => /orP [] //.
+          rewrite in_set /=.
+          
+        
+    End Correctness.    
+        
+  End Minimalization.
+  
+
   Section ToMN.
     Variable A: dfa char.
     Definition f : Fin_eq_cls A := [ fun w => last (dfa_s0 A) (dfa_run A w) ].
 
-    Lemma f_correct: MH_rel_ref _ (dfa_lang A) f.
+    Lemma f_correct: MN_rel _ (dfa_lang A) f.
     Proof.
       move => w1 w2.
       rewrite /f /=.
